examples/all_exists/PCsat/Ti_GNI_HTT/prog.rl
@@ -17,38 +17,38 @@ specialized with high1 and high2
 */
 
 interface I =
-  meth prog (n:int) : int
-    effects { rd n }
+  meth prog (low:int) : int
 end
 
 module A : I =
-  meth prog (n: int) : int
+  meth prog (low: int) : int
 end
 
 
 
 bimodule FREL (A | A) =
-  meth prog (l: int |  l: int) : (int | int)
-  requires { l =:= l }
+  meth prog (low: int |  low: int) : (int | int)
+  requires { low =:= low }
   ensures { result =:= result }
  =
+    Var x: int | x: int in
 
-    Var a: bool | a: bool in
-
-    (havoc result | skip);
-    (if (result <= l)
+    (havoc x | skip);
+    (if (x >= low)
       then
-        result := l;
+        x := x;
       else
-        result := result;
+        x := low;
       end | skip);
 
-    HavocR result { result =:= result } ;
+    HavocR x { x =:= x } ;
 
-    (skip | if (result <= l)
+    (skip | if (x >= low)
             then
-              result := l;
+              x := x;
             else
-              result := result;
+              x := low;
             end);
+
+    |_ result := x _|;
 end
